valueScript.sml
@@ -728,4 +728,135 @@ Proof
   rw[IN_DEF,freevars_v_def]
 QED
 
+Definition v_finite_def:
+  v_finite v = ltree_finite(v_rep v)
+End
+
+Theorem v_finite:
+  v_finite(Atom a) ∧
+  v_finite(Closure x body) ∧
+  v_finite(Error) ∧
+  v_finite(Diverge) ∧
+  v_finite(Constructor s l) = EVERY v_finite l
+Proof
+  rw[v_finite_def,Atom_def,Closure_def,Error_def,Diverge_def,Constructor_def,GSYM v_repabs_imp,
+     v_rep_ok_Atom,v_rep_ok_Closure,v_rep_ok_Error,v_rep_ok_Diverge,v_rep_ok_Constructor] >>
+  rw[Atom_rep_def,Closure_rep_def,Diverge_rep_def,Error_rep_def,Constructor_rep_def,
+     ltree_finite_cases] >>
+  simp[EVERY_MAP,GSYM v_finite_def] >>
+  metis_tac[]
+QED
+
+Theorem v_finite_ind:
+  (∀a. P(Atom a)) ∧
+  (∀x body. P(Closure x body)) ∧
+  (P Diverge) ∧
+  (P Error) ∧
+  (∀s vl. EVERY P vl ⇒ P (Constructor s vl))
+  ⇒
+  ∀t. v_finite t ⇒ P t
+Proof
+  strip_tac >>
+  ‘∀x. ltree_finite x ⇒ ∀t. x = v_rep t ⇒ P (v_abs (v_rep t))’
+   suffices_by(gvs[v_finite_def,PULL_FORALL,v_absrep]) >>
+  ho_match_mp_tac ltree_finite_ind >>
+  rw[v_absrep] >>
+  rename1 ‘v_rep t’ >>
+  Cases_on ‘t’ >> gvs[Constructor_def,GSYM v_repabs_imp,v_rep_ok_Constructor] >>
+  gvs[Constructor_rep_def,EVERY_MAP] >>
+  first_x_assum match_mp_tac >>
+  match_mp_tac (MP_CANON EVERY_MONOTONIC) >>
+  first_x_assum(irule_at (Pos last)) >>
+  rw[]
+QED
+
+Definition v_take_def:
+  v_take (n:num) t =
+    case t of
+      Constructor s vl =>
+        if n = 0 then Constructor s []
+        else
+          Constructor s (MAP (v_take (n-1)) vl)
+    | v => v
+End
+
+Theorem v_take_finite:
+  ∀n v. v_finite(v_take n v)
+Proof
+  Induct >> rw[v_finite,Once v_take_def] >>
+  BasicProvers.TOP_CASE_TAC >> rw[v_finite] >>
+  rw[EVERY_MEM,MEM_MAP] >> simp[]
+QED
+
+Theorem v_take_add:
+  ∀n v x.
+    v_take n v = v ⇒
+    v_take (n + x) v = v
+Proof
+  ho_match_mp_tac v_take_ind >>
+  ntac 3 strip_tac >>
+  PURE_ONCE_REWRITE_TAC[v_take_def] >>
+  rw[] >> BasicProvers.TOP_CASE_TAC >> gvs[] >>
+  Cases_on ‘n = 0’ >> gvs[] >>
+  CONV_TAC(RHS_CONV(PURE_ONCE_REWRITE_CONV [GSYM(cj 1 MAP_ID)])) >>
+  qpat_x_assum ‘_ = _’ (mp_tac o CONV_RULE(RHS_CONV(PURE_ONCE_REWRITE_CONV [GSYM(cj 1 MAP_ID)]))) >>
+  SIMP_TAC std_ss [MAP_EQ_f] >>
+  rw[]
+QED
+
+Theorem v_take_finite:
+  ∀v. v_finite v ⇔ ∃n. v_take n v = v
+Proof
+  simp[EQ_IMP_THM,FORALL_AND_THM] >>
+  reverse conj_tac >- metis_tac[v_take_finite] >>
+  ho_match_mp_tac v_finite_ind >> rw[] >>
+  rw[Once v_take_def] >>
+  Q.REFINE_EXISTS_TAC ‘SUC _’ >> rw[] >>
+  pop_assum mp_tac >> Induct_on ‘vl’ >> rw[] >>
+  res_tac >>
+  rename1 ‘MAP (λa. v_take m a)’ >>
+  qexists_tac ‘MAX n m’ >>
+  rw[MAX_DEF,NOT_LESS]
+  >- (imp_res_tac LESS_ADD >> gvs[v_take_add]) >>
+  gvs[NOT_LESS] >>
+  imp_res_tac LESS_EQUAL_ADD >>
+  gvs[] >>
+  CONV_TAC(RHS_CONV(PURE_ONCE_REWRITE_CONV [GSYM(cj 1 MAP_ID)])) >>
+  pop_assum (mp_tac o CONV_RULE(RHS_CONV(PURE_ONCE_REWRITE_CONV [GSYM(cj 1 MAP_ID)]))) >>
+  SIMP_TAC std_ss [MAP_EQ_f] >>
+  rw[v_take_add]
+QED
+
+(* v_bisimulation in implication form. Much easier to apply that way. *)
+Theorem v_coinduct:
+  ∀R. (∀v3 v4. R v3 v4 ⇒
+               (∃a. v3 = Atom a ∧ v4 = Atom a) ∨
+               (∃s vs3 vs4.
+                  v3 = Constructor s vs3 ∧
+                  v4 = Constructor s vs4 ∧
+                  LIST_REL R vs3 vs4) ∨
+               (∃s e. v3 = Closure s e ∧ v4 = Closure s e) ∨
+               (v3 = Diverge ∧ v4 = Diverge) ∨
+               (v3 = Error ∧ v4 = Error)) ⇒
+      ∀v1 v2. R v1 v2 ⇒ v1 = v2
+Proof
+  rw[] >> simp[Once v_bisimulation] >>
+  goal_assum drule >>
+  first_x_assum MATCH_ACCEPT_TAC
+QED
+
+Theorem v_take_lemma:
+  ∀v1 v2. v1 = v2 ⇔ ∀n. v_take n v1 = v_take n v2
+Proof
+  simp[EQ_IMP_THM,FORALL_AND_THM] >>
+  ho_match_mp_tac v_coinduct >>
+  rw[] >>
+  ‘∀n. v_take (SUC n) v1 = v_take (SUC n) v2’ by metis_tac[] >>
+  last_x_assum kall_tac >>
+  pop_assum(mp_tac o PURE_ONCE_REWRITE_RULE[v_take_def]) >>
+  ntac 2 (BasicProvers.TOP_CASE_TAC) >> rw[] >>
+  gvs[FORALL_AND_THM,MAP_EQ_EVERY2] >>
+  gvs[LIST_REL_EL_EQN]
+QED
+
 val _ = export_theory ();
